preliminaries

automata.v
@@ -1,28 +1,146 @@
 Require Import Ensembles.
 Require Import List.
-Require Import Nat. 
+Require Import Nat.
+Import ListNotations.
+Require Import Coq.Structures.Equalities.
 
-Definition word char := list char.
+
+Inductive word (char : Set) :=
+  | Eps : word char
+  | Concat : char -> word char -> word char.
+
+Scheme Equality for word.
+
+
+Notation "'Eps'" := (Eps _).
+
+Notation "w1 ++ w2" := (Concat _ w1 w2) (at level 60, right associativity).
+
+Fixpoint length {char : Set} (w : word char) : nat :=
+  match w with
+  | Eps => 0
+  | a ++ w' => S (length w')
+  end.
+
+Definition eq_word char : forall x y : word char, {x = y} + {x <> y}.
+Proof.
+  intros.
+  decide equality.
+  induction w.
+  (*TODO*)
+  admit.
+
+Defined.
+
 
 Definition dlang char := word char -> Prop.
 
-Inductive downset (n: nat) : Set := admit.
+Definition eq_dlang char : forall x y : dlang char, {x = y} + {x <> y}.
+Proof.
+  unfold dlang.
+  intros.
+  decide equality.
+  admit.
 
-Check nat.
 
-(*TODO*)
-Definition incl {n : nat} (s : downset n) : nat := n. 
 
-Check firstn.
 
-Definition lastn{A} (n : nat) (l : list A) := firstn n (rev l).
 
-Definition concat{char : Set} (L1 L2 : dlang char) : dlang char :=
-  fun v =>
-    
-      exists i : (downset (length v + 1)), L1 (firstn (incl i) v) /\ L2 (lastn (incl i) v)
-    
-.
+(*Curried definition of the transition function*)
 
-Lemma concP (L1 L2 : dlang char) {w : word char} :
-  reflect ()
+
+Record NFA := mkNFA {
+  nstates : Set
+  ; nalphabet : Set
+  ; ntransition : nstates -> option nalphabet -> nstates -> Prop
+  ; ninitial : nstates -> Prop
+  ; nfinal : nstates -> Prop
+}.
+
+
+
+Record DFA := mkDFA {
+  dstates : Set
+  ; dalphabet : Set
+  ; dtransition : dstates -> dalphabet -> dstates
+  ; dinitial : dstates
+  ; dfinal : dstates -> Prop
+}.
+
+Fixpoint DRecognizedWord (d : DFA) (w : word (dalphabet d))  : Prop :=
+  let
+    fix aux (w' : word (dalphabet d)) (q : dstates d) : Prop :=
+      match w' with
+      | Eps => dfinal d q
+      |  a ++ w'' =>  aux w'' (dtransition d q a)
+      end
+    in
+  aux w (dinitial d).
+
+Fixpoint NRecognizedWord (n : NFA) (w : word (nalphabet n))  : Prop :=
+  let
+    fix aux (w' : word (nalphabet n)) (q : nstates n) : Prop :=
+      match w' with
+      | Eps => nfinal n q
+      |  a ++ w'' => exists q': nstates n, ntransition n q (Some a) q' ->  aux w'' q'
+      end
+    in
+  exists q0: nstates n, ninitial n q0 -> aux w q0.
+
+Definition DRecognizedLanguage (d : DFA) : dlang (dalphabet d) :=
+  DRecognizedWord d.
+
+Definition NRecognizedLanguage (n : NFA) : dlang (nalphabet n) :=
+  NRecognizedWord n.
+
+Definition DFAtoNFA (d : DFA) : NFA :=
+  {|
+    nalphabet := dalphabet d;
+    nstates := dstates d;
+    ntransition := fun q a q' =>
+      match a with
+      | None => False
+      | Some a => dtransition d q a = q'
+      end;
+    ninitial := fun q => q = dinitial d;
+    nfinal := dfinal d
+  |}.
+
+Lemma rec_same_dfa_to_nfa :
+  forall d : DFA, DRecognizedLanguage d = NRecognizedLanguage (DFAtoNFA d).
+Proof.
+  intros d.
+  unfold DRecognizedLanguage, NRecognizedLanguage.
+  unfold DRecognizedWord, NRecognizedWord.
+  unfold DFAtoNFA.
+  admit.
+
+
+
+Record CFG := mkCFG
+{
+  nonterminals : Set;
+  terminals : Set;
+  production : nonterminals -> word (sum nonterminals terminals);
+  start : nonterminals
+}.
+
+Definition CFGRecognizedWord (c : CFG) (w : word (terminals c)) :=
+  admit.
+
+Definition CFGRecognizedLanguage (c : CFG) : dlang (terminals c) :=
+  CFGRecognizedWord c.
+
+Definition inCNF (c : CFG) : Prop :=
+  forall n : nonterminals c,
+  length (production c n) <= 2.
+
+Fixpoint CFGtoCNF (c : CFG) : CFG :=
+  admit.
+
+Lemma CFG_to_CNF_is_correct :
+  forall c : CFG, inCNF (CFGtoCNF c).
+
+Lemma rec_same_CFG_CNF :
+  forall c : CFG,
+  CFGRecognizedLanguage (CFGtoCNF c) = CFGRecognizedLanguage c.
